language_formalisation/type_system/subtyping.v
@@ -17,14 +17,23 @@ Inductive vsubtype : vtype -> vtype -> Prop :=
     csubtype C' C -> csubtype D D' -> vsubtype (TyHandler C D) (TyHandler C' D')
 
 with csubtype : ctype -> ctype -> Prop  :=
-| Csubty A A' Σ Σ' E : 
-    vsubtype A A' -> sig_subtype Σ Σ' -> csubtype (CTy A Σ E) (CTy A' Σ' E)
+| Csubty A A' Σ Σ' E E': 
+    vsubtype A A' -> sig_subtype Σ Σ' -> eqs_subtype E E' ->
+    csubtype (CTy A Σ E) (CTy A' Σ' E')
 
 with sig_subtype : sig -> sig -> Prop :=
-| SigØsubty : sig_subtype SigØ SigØ
+| SigØsubty Σ: sig_subtype SigØ Σ
 | SigUsubty Σ Σ' op A B A' B' : 
-    sig_subtype Σ Σ' -> vsubtype A' A -> vsubtype B B' ->
-    sig_subtype (SigU Σ op A B) (SigU Σ' op A' B')
+    sig_subtype Σ Σ' -> 
+    get_op_type Σ op = None -> get_op_type Σ' op = Some (A', B') -> 
+    vsubtype A' A -> vsubtype B B' ->
+    sig_subtype (SigU Σ op A B) Σ'
+
+with eqs_subtype : eqs -> eqs -> Prop :=
+| EqsØsubty E: eqs_subtype EqsØ E
+| EqsUsubty E E' Γ Z T1 T2 : 
+    eqs_subtype E E' -> eqs_contain_eq E' Γ Z T1 T2 ->
+    eqs_subtype (EqsU E Γ Z T1 T2) E'
 .
 
 Inductive ctx_subtype : ctx -> ctx -> Prop :=
@@ -32,109 +41,3 @@ Inductive ctx_subtype : ctx -> ctx -> Prop :=
 | CtxUsubty Γ Γ' A A' : 
     ctx_subtype Γ Γ' -> vsubtype A A' -> ctx_subtype (CtxU Γ A) (CtxU Γ' A')
 .
-
-Ltac inv H := inversion H; clear H; subst.
-
-(* Weird notation for SPEED! *)
-Fixpoint vsubtype_trans A1 A2 A3 
-  (A12 : vsubtype A1 A2) {struct A12} : vsubtype A2 A3 -> vsubtype A1 A3
-with vsubtype_trans_rev A1 A2 A3
-  (A21 : vsubtype A2 A1) {struct A21} : vsubtype A3 A2 -> vsubtype A3 A1
-with csubtype_trans C1 C2 C3
-  (C12 : csubtype C1 C2) {struct C12} : csubtype C2 C3 -> csubtype C1 C3
-with csubtype_trans_rev C1 C2 C3 
-  (C21 : csubtype C2 C1) {struct C21} : csubtype C3 C2 -> csubtype C3 C1
-with sig_subtype_trans Σ1 Σ2 Σ3 
-  (S12 : sig_subtype Σ1 Σ2) {struct S12} : sig_subtype Σ2 Σ3 -> 
-  sig_subtype Σ1 Σ3
-with sig_subtype_trans_rev Σ1 Σ2 Σ3
-  (S21 : sig_subtype Σ2 Σ1) (S32 : sig_subtype Σ3 Σ2) {struct S21} : 
-  sig_subtype Σ3 Σ1.
-Proof.
-{
-clear sig_subtype_trans sig_subtype_trans_rev.
-intros A23; destruct A12; try assumption; inv A23.
-+ apply VsubtyTyΣ.
-  - eapply vsubtype_trans. exact A12_1. assumption.
-  - eapply vsubtype_trans. exact A12_2. assumption.
-+ apply VsubtyTyΠ.
-  - eapply vsubtype_trans. exact A12_1. assumption.
-  - eapply vsubtype_trans. exact A12_2. assumption.
-+ apply VsubtyFun.
-  - eapply vsubtype_trans_rev. exact A12. assumption. 
-  - eapply csubtype_trans. exact H. assumption.
-+ apply VsubtyHandler.
-  - eapply csubtype_trans_rev. exact H. assumption. 
-  - eapply csubtype_trans. exact H0. assumption.
-}{
-clear sig_subtype_trans sig_subtype_trans_rev.
-intros A32; destruct A21; try assumption; inv A32.
-+ apply VsubtyTyΣ.
-  - eapply vsubtype_trans_rev. exact A21_1. assumption.
-  - eapply vsubtype_trans_rev. exact A21_2. assumption.
-+ apply VsubtyTyΠ.
-  - eapply vsubtype_trans_rev. exact A21_1. assumption.
-  - eapply vsubtype_trans_rev. exact A21_2. assumption.
-+ apply VsubtyFun.
-  - eapply vsubtype_trans. exact A21. assumption. 
-  - eapply csubtype_trans_rev. exact H. assumption.
-+ apply VsubtyHandler.
-  - eapply csubtype_trans. exact H. assumption. 
-  - eapply csubtype_trans_rev. exact H0. assumption.
-}{
-clear vsubtype_trans_rev csubtype_trans csubtype_trans_rev sig_subtype_trans_rev.
-intros C23; destruct C12. inv C23.
-apply Csubty.
-- eapply vsubtype_trans. exact H. assumption.
-- eapply sig_subtype_trans. exact H0. assumption.
-}{
-clear vsubtype_trans csubtype_trans csubtype_trans_rev sig_subtype_trans.
-intros C32; destruct C21. inv C32.
-apply Csubty.
-- eapply vsubtype_trans_rev. exact H. assumption.
-- eapply sig_subtype_trans_rev. exact H0. assumption.
-}{
-clear csubtype_trans csubtype_trans_rev.
-clear sig_subtype_trans_rev.
-intros S23. destruct S12. inv S23.
-apply SigØsubty.
-inv S23. apply SigUsubty. 
-+ eapply sig_subtype_trans. exact S12. assumption.
-+ eapply vsubtype_trans_rev. exact H. assumption.
-+ eapply vsubtype_trans. exact H0. assumption.
-}{
-clear csubtype_trans csubtype_trans_rev.
-clear sig_subtype_trans.
-destruct S21. inv S32.
-apply SigØsubty.
-inv S32. apply SigUsubty. 
-+ eapply sig_subtype_trans_rev. exact S21. assumption.
-+ eapply vsubtype_trans. exact H. assumption.
-+ eapply vsubtype_trans_rev. exact H0. assumption.
-}
-Qed.
-
-
-Lemma vsubty_refl v : vsubtype v v
-with csubty_refl c : csubtype c c
-with sigsubty_refl Σ : sig_subtype Σ Σ
-with ctx_subty_refl Γ : ctx_subtype Γ Γ.
-Proof.
-{induction v.
-+ apply VsubtyUnit.
-+ apply VsubtyInt.
-+ apply VsubtyTyØ.
-+ apply VsubtyTyΣ; assumption.
-+ apply VsubtyTyΠ; assumption.
-+ apply VsubtyFun. assumption. apply csubty_refl.
-+ apply VsubtyHandler; apply csubty_refl.
-}{ destruct c. apply Csubty.
-apply vsubty_refl. apply sigsubty_refl.
-}{ induction Σ.
-+ apply SigØsubty.
-+ apply SigUsubty; try assumption || apply vsubty_refl.
-}{induction Γ.
-+ apply CtxØsubty.
-+ apply CtxUsubty. assumption. apply vsubty_refl.
-}
-Qed.
