language_formalisation/type_system/subtyping_lemmas.v
@@ -2,8 +2,301 @@
 (* Add LoadPath "C:\Users\Ziga\Documents\Ziga_podatki\PHD\language_formalisation\type_system". *)
 Add LoadPath "E:\Ziga_Podatki\faks\PHD\language_formalisation\syntax".
 Add LoadPath "E:\Ziga_Podatki\faks\PHD\language_formalisation\type_system".
+Add LoadPath "E:\Ziga_Podatki\faks\PHD\language_formalisation\substitution".
 
-Require Import syntax declarational.
+Require Import syntax declarational wellfounded_lemmas.
+
+
+Ltac inv H := inversion H; clear H; subst.
+
+(* ========================== Auxiliary Lemmas ========================== *)
+
+Lemma sig_subtype_gets_Some Σ Σ' op A B :
+  sig_subtype Σ Σ' -> get_op_type Σ op = Some (A, B) -> exists A' B', 
+  get_op_type Σ' op = Some (A', B') /\ vsubtype A' A /\ vsubtype B B'.
+Proof.
+intros sty gets. induction sty.
++ simpl in gets. discriminate.
++ simpl in gets. destruct (op == op0).
+  - injection gets. intros. subst. exists A'. exists B'.
+    constructor. assumption. constructor; assumption.
+  - apply IHsty in gets. assumption.
+Qed.
+
+Lemma sig_subtype_gets_None Σ Σ' op :
+  sig_subtype Σ Σ' -> get_op_type Σ' op = None -> get_op_type Σ op = None.
+Proof.
+intros sty gets. induction sty.
++ simpl. reflexivity.
++ simpl. destruct (op == op0).
+  - rewrite e in *. rewrite gets in H0. discriminate.
+  - apply IHsty. assumption.
+Qed.
+
+Lemma sig_subtype_extend Σ Σ' op A B :
+  sig_subtype Σ Σ' -> wf_sig (SigU Σ' op A B) -> sig_subtype Σ (SigU Σ' op A B).
+Proof.
+intros.
+induction H.
++ apply SigØsubty.
++ eapply SigUsubty.
+  - apply IHsig_subtype. assumption.
+  - assumption.
+  - inv H0. simpl. destruct (op0 == op). 
+    * rewrite e in *. rewrite H2 in H10. discriminate.
+    * exact H2.
+  - assumption.
+  - assumption.
+Qed.
+
+Lemma sig_subtype_sigempty Σ : sig_subtype Σ SigØ -> Σ = SigØ.
+Proof.
+intro subty.
+inv subty. reflexivity.
+simpl in H1. discriminate.
+Qed.
+
+Lemma eqs_subtype_extend E E' Σ Γ Z T1 T2 :
+  eqs_subtype E E' -> wf_eqs (EqsU E' Γ Z T1 T2) Σ ->
+  eqs_subtype E (EqsU E' Γ Z T1 T2).
+Proof.
+intros.
+induction H.
++ apply EqsØsubty.
++ eapply EqsUsubty.
+  - apply IHeqs_subtype. assumption.
+  - simpl. right. assumption.
+Qed.
+
+(* ========================== Basic Properties ========================== *)
+
+Lemma vsubty_refl v : wf_vtype v -> vsubtype v v
+with csubty_refl c : wf_ctype c -> csubtype c c
+with sig_subty_refl Σ : wf_sig Σ -> sig_subtype Σ Σ
+with eqs_subty_refl E Σ : wf_eqs E Σ -> eqs_subtype E E
+with ctx_subty_refl Γ : wf_ctx Γ -> ctx_subtype Γ Γ.
+Proof.
+{intros; induction v; inv H.
++ apply VsubtyUnit.
++ apply VsubtyInt.
++ apply VsubtyTyØ.
++ apply VsubtyTyΣ; auto.
++ apply VsubtyTyΠ; auto.
++ apply VsubtyFun. apply IHv. assumption. apply csubty_refl. assumption.
++ apply VsubtyHandler; apply csubty_refl; assumption.
+}{ destruct c. intros. inv H. apply Csubty.
+apply vsubty_refl. assumption. 
+apply sig_subty_refl. assumption.
+eapply eqs_subty_refl. exact H5.
+}{ 
+intros; induction Σ.
++ apply SigØsubty.
++ eapply SigUsubty.
+  - apply sig_subtype_extend. apply IHΣ. inv H. assumption. assumption.
+  - inv H. assumption.
+  - simpl. destruct (o==o). reflexivity. destruct n. reflexivity.
+  - apply vsubty_refl. inv H. assumption.
+  - apply vsubty_refl. inv H. assumption.
+}{induction E; intros.
++ apply EqsØsubty.
++ apply EqsUsubty. inv H. eapply eqs_subtype_extend. 
+  - apply IHE. assumption.
+  - apply WfEqsU. exact H6. assumption. assumption.
+  - simpl. left. auto.
+}{induction Γ; intros.
++ apply CtxØsubty.
++ apply CtxUsubty; inv H. apply IHΓ. assumption. apply vsubty_refl. assumption.
+}
+Qed.
+
+(* stupid auxiliary definition for reverse sigma transitivity *)
+Fixpoint remove_op_from_sig Σ op :=
+  match Σ with
+  | SigØ => SigØ
+  | SigU Σ' op' A B => 
+      if (op == op') then Σ' 
+      else SigU (remove_op_from_sig Σ' op) op' A B
+end.
+
+Lemma remove_op_get_op Σ op op' :
+  op <> op' -> get_op_type (remove_op_from_sig Σ op) op' = get_op_type Σ op'.
+Proof.
+intros. induction Σ.
++ auto.
++ simpl. destruct (op'==o); destruct (op==o).
+  - subst. destruct H. reflexivity.
+  - simpl. destruct (op'==o). reflexivity. subst. destruct n0. auto.
+  - reflexivity.
+  - simpl. destruct (op'==o). subst. destruct n. auto. assumption.
+Qed.
+
+Lemma remove_op_wf Σ op : wf_sig Σ -> wf_sig (remove_op_from_sig Σ op).
+Proof.
+intros. induction H.
++ simpl. apply WfSigØ.
++ simpl in *. destruct (op == op0). assumption. apply WfSigU.
+  all: try assumption. rewrite remove_op_get_op; assumption.
+Qed.
+
+Lemma sig_remove_op_intro Σ Σ' op A B :
+  wf_sig Σ' -> sig_subtype Σ (SigU Σ' op A B) -> 
+  sig_subtype (remove_op_from_sig Σ op) Σ'.
+Proof.
+intros wf' orig.
+induction Σ.
++ simpl. apply SigØsubty.
++ simpl. destruct (op==o).
+  assert (forall Σ op, get_op_type Σ op = None -> remove_op_from_sig Σ op = Σ).
+  { intros. induction Σ0. simpl. reflexivity. simpl in *.
+    destruct (op0==o0). discriminate. f_equal. apply IHΣ0. assumption. }
+  - inv orig. rewrite H in IHΣ. apply IHΣ. all: assumption.
+  - inv orig. eapply SigUsubty. apply IHΣ. assumption.
+    * rewrite remove_op_get_op. assumption. assumption.
+    * simpl in H6. destruct (o==op). subst. destruct n. reflexivity.
+      exact H6.
+    * assumption.
+    * assumption.
+Qed.
+
+Lemma sig_remove_op_elim Σ Σ' op A B :
+  get_op_type Σ op = Some (A, B) ->
+  sig_subtype (SigU (remove_op_from_sig Σ op) op A B) Σ' ->
+  sig_subtype Σ Σ'.
+Proof.
+Admitted.
+
+(* Weird notation for SPEED! *)
+Fixpoint vsubtype_trans A1 A2 A3 
+  (A12 : vsubtype A1 A2) {struct A12} : 
+  wf_vtype A1 -> wf_vtype A2 -> wf_vtype A3 -> 
+  vsubtype A2 A3 -> 
+  vsubtype A1 A3
+with vsubtype_trans_rev A1 A2 A3
+  (A21 : vsubtype A2 A1) {struct A21} : 
+  wf_vtype A1 -> wf_vtype A2 -> wf_vtype A3 -> 
+  vsubtype A3 A2 ->
+  vsubtype A3 A1
+with csubtype_trans C1 C2 C3
+  (C12 : csubtype C1 C2) {struct C12} : 
+  wf_ctype C1 -> wf_ctype C2 -> wf_ctype C3 -> 
+  csubtype C2 C3 -> 
+  csubtype C1 C3
+with csubtype_trans_rev C1 C2 C3 
+  (C21 : csubtype C2 C1) {struct C21} : 
+  wf_ctype C1 -> wf_ctype C2 -> wf_ctype C3 -> 
+  csubtype C3 C2 -> 
+  csubtype C3 C1
+with sig_subtype_trans Σ1 Σ2 Σ3 
+  (S12 : sig_subtype Σ1 Σ2) {struct S12} : 
+  wf_sig Σ1 -> wf_sig Σ2 -> wf_sig Σ3 ->  
+  sig_subtype Σ2 Σ3 -> 
+  sig_subtype Σ1 Σ3
+with sig_subtype_trans_rev Σ1 Σ2 Σ3
+  (S21 : sig_subtype Σ2 Σ1) {struct S21} : 
+  wf_sig Σ1 -> wf_sig Σ2 -> wf_sig Σ3 ->  sig_subtype Σ3 Σ2 ->
+  sig_subtype Σ3 Σ1
+with eqs_subtype_trans E1 E2 E3 Σ1 Σ2 Σ3 
+  (E12 : eqs_subtype E1 E2) {struct E12} : 
+  wf_eqs E1 Σ1 -> wf_eqs E2 Σ2 -> wf_eqs E3 Σ3 ->  
+  eqs_subtype E2 E3 -> 
+  eqs_subtype E1 E3
+with eqs_subtype_trans_rev E1 E2 E3 Σ1 Σ2 Σ3
+  (E21 : eqs_subtype E2 E1) {struct E21} : 
+  wf_eqs E1 Σ1 -> wf_eqs E2 Σ2 -> wf_eqs E3 Σ3 ->  eqs_subtype E3 E2 ->
+  eqs_subtype E3 E1.
+Proof.
+{
+clear sig_subtype_trans sig_subtype_trans_rev.
+clear eqs_subtype_trans eqs_subtype_trans_rev.
+intros wf1 wf2 wf3 A23; destruct A12; try assumption; 
+inv A23; inv wf1; inv wf2; inv wf3. 
++ apply VsubtyTyΣ.
+  - eapply vsubtype_trans. exact A12_1. all: assumption.
+  - eapply vsubtype_trans. exact A12_2. all: assumption.
++ apply VsubtyTyΠ.
+  - eapply vsubtype_trans. exact A12_1. all: assumption.
+  - eapply vsubtype_trans. exact A12_2. all: assumption.
++ apply VsubtyFun.
+  - eapply vsubtype_trans_rev. exact A12. all: assumption. 
+  - eapply csubtype_trans. exact H. all: assumption.
++ apply VsubtyHandler.
+  - eapply csubtype_trans_rev. exact H. all: assumption. 
+  - eapply csubtype_trans. exact H0. all: assumption.
+}{
+clear sig_subtype_trans sig_subtype_trans_rev.
+clear eqs_subtype_trans eqs_subtype_trans_rev.
+intros wf1 wf2 wf3 A32; destruct A21; try assumption;
+inv A32; inv wf1; inv wf2; inv wf3. 
++ apply VsubtyTyΣ.
+  - eapply vsubtype_trans_rev. exact A21_1. all: assumption.
+  - eapply vsubtype_trans_rev. exact A21_2. all: assumption.
++ apply VsubtyTyΠ.
+  - eapply vsubtype_trans_rev. exact A21_1. all: assumption.
+  - eapply vsubtype_trans_rev. exact A21_2. all: assumption.
++ apply VsubtyFun.
+  - eapply vsubtype_trans. exact A21. all: assumption. 
+  - eapply csubtype_trans_rev. exact H. all: assumption.
++ apply VsubtyHandler.
+  - eapply csubtype_trans. exact H. all: assumption. 
+  - eapply csubtype_trans_rev. exact H0. all: assumption.
+}{
+clear vsubtype_trans_rev csubtype_trans csubtype_trans_rev.
+clear sig_subtype_trans_rev eqs_subtype_trans_rev.
+intros wf1 wf2 wf3 C23; destruct C12. 
+inv C23; inv wf1; inv wf2; inv wf3. 
+apply Csubty.
+- eapply vsubtype_trans. exact H. all: assumption.
+- eapply sig_subtype_trans. exact H0. all: assumption.
+- eapply eqs_subtype_trans. all: eauto.
+}{
+clear vsubtype_trans csubtype_trans csubtype_trans.
+clear sig_subtype_trans eqs_subtype_trans.
+intros wf1 wf2 wf3 C32; destruct C21. 
+inv C32; inv wf1; inv wf2; inv wf3. 
+apply Csubty.
+- eapply vsubtype_trans_rev. exact H. all: assumption.
+- eapply sig_subtype_trans_rev. exact H0. all: assumption.
+- eapply eqs_subtype_trans_rev. all: eauto.
+}{
+clear csubtype_trans csubtype_trans_rev eqs_subtype_trans eqs_subtype_trans_rev.
+intros wf1 wf2 wf3 S23. destruct S12.
+apply SigØsubty.
+apply (sig_subtype_gets_Some Σ' Σ3) in H0 as H0'. destruct H0' as [A'' [B'' [g]]].
+eapply SigUsubty.
++ eapply sig_subtype_trans. exact S12. inv wf1. all : assumption.
++ assumption.
++ exact g.
++ clear sig_subtype_trans vsubtype_trans.
+  destruct H3. eapply vsubtype_trans_rev. exact H1.
+  - inv wf1. assumption.
+  - apply get_op_type_wf in H0. destruct H0. assumption. assumption.
+  - apply get_op_type_wf in g. destruct g. assumption. assumption.
+  - assumption.
++ clear sig_subtype_trans vsubtype_trans_rev.
+  destruct H3. eapply vsubtype_trans. exact H2.
+  - inv wf1. assumption.
+  - apply get_op_type_wf in H0. destruct H0. assumption. assumption.
+  - apply get_op_type_wf in g. destruct g. assumption. assumption.
+  - assumption.
++ assumption.
+}{
+(* clear csubtype_trans csubtype_trans_rev eqs_subtype_trans eqs_subtype_trans_rev.
+clear sig_subtype_trans.
+intros wf1 wf2 wf3 S32. destruct S21.
+apply sig_subtype_sigempty in S32. subst. apply SigØsubty.
+apply sig_remove_op_intro in S32 as S32'. 2: (inv wf2; assumption).
+specialize (remove_op_wf Σ3 op wf3) as wfr. inv wf2.
+specialize (sig_subtype_trans_rev _ _ _ S21 wf1 H7 wfr S32') as rec.
+clear sig_subtype_trans_rev.
+destruct (get_op_type Σ3 op) eqn: gets.
+- destruct p. eapply sig_remove_op_elim. exact gets.
+  inv S32. simpl. *)
+
+
+}
+Qed.
+
+
 
 Fixpoint ctx_subtype_get Γ Γ' A num
   (ctx_sty : ctx_subtype Γ Γ') {struct ctx_sty}:
